examples/pseudo_bool/array/colourProgScript.sml
@@ -35,7 +35,7 @@ Definition parse_annots_def:
   (parse_annots [] acc = SOME acc) ∧
   (parse_annots (s::ss) acc =
   case parse_annot s of
-   (SOME annot,line) =>
+   ([annot],line) =>
      parse_annots ss (annot::acc)
   | _ => NONE)
 End
@@ -175,7 +175,7 @@ Theorem parse_and_enc_spec:
             INT))
             (LIST_TYPE
               (PAIR_TYPE
-              (OPTION_TYPE STRING_TYPE)
+              (LIST_TYPE STRING_TYPE)
               (PAIR_TYPE (PBC_PBHD_TYPE STRING_TYPE) (PAIR_TYPE (LIST_TYPE (PAIR_TYPE INT (PBC_LIT_TYPE STRING_TYPE))) INT))))
             ) res v ∧
        case res of
@@ -203,7 +203,7 @@ QED
 Definition mk_prob_def:
   mk_prob objf = (NONE,objf):mlstring list option #
     ((int # mlstring pbc$lit) list # int) option #
-    (mlstring option # (mlstring pbhd # (int # mlstring pbc$lit) list # int)) list
+    (mlstring list # (mlstring pbhd # (int # mlstring pbc$lit) list # int)) list
 End
 
 val res = translate mk_prob_def;
