examples/pseudo_bool/array/mccisProgScript.sml
@@ -61,7 +61,7 @@ Theorem parse_and_enc_spec:
             INT))
             (LIST_TYPE
               (PAIR_TYPE
-              (OPTION_TYPE STRING_TYPE)
+              (LIST_TYPE STRING_TYPE)
               (PAIR_TYPE (PBC_PBHD_TYPE STRING_TYPE) (PAIR_TYPE (LIST_TYPE (PAIR_TYPE INT (PBC_LIT_TYPE STRING_TYPE))) INT))))
             )) res v ∧
        case res of
@@ -158,7 +158,7 @@ val res = translate map_concl_to_string_def;
 Definition mk_prob_def:
   mk_prob objf = (NONE,objf):mlstring list option #
     ((int # mlstring pbc$lit) list # int) option #
-    (mlstring option #
+    (mlstring list #
       (mlstring pbhd # (int # mlstring pbc$lit) list # int)) list
 End
 
