examples/pseudo_bool/array/mcliqueProgScript.sml
@@ -39,7 +39,7 @@ Theorem parse_and_enc_spec:
             (OPTION_TYPE (LIST_TYPE STRING_TYPE))
             (LIST_TYPE
               (PAIR_TYPE
-              (OPTION_TYPE STRING_TYPE)
+              (LIST_TYPE STRING_TYPE)
               (PAIR_TYPE (PBC_PBHD_TYPE STRING_TYPE) (PAIR_TYPE (LIST_TYPE (PAIR_TYPE INT (PBC_LIT_TYPE STRING_TYPE))) INT))))
             ) res v ∧
        case res of
@@ -116,7 +116,7 @@ val res = translate map_concl_to_string_def;
 Definition mk_prob_def:
   mk_prob (pres,f) = (pres,NONE,f):mlstring list option #
     ((int # mlstring pbc$lit) list # int) option #
-    (mlstring option # (mlstring pbhd # (int # mlstring pbc$lit) list # int)) list
+    (mlstring list # (mlstring pbhd # (int # mlstring pbc$lit) list # int)) list
 End
 
 val res = translate mk_prob_def;
